com.io7m.calino.specification/src/main/coq/Calino/Compression.v
@@ -1,7 +1,7 @@
 Require Import Coq.Strings.String.
 Require Import Coq.Unicode.Utf8_core.
 
-Require Import Calino.Descriptor.
+Require Import Calino.Descriptor.  
 
 Inductive compressionMethod : Set :=
   | CompressionUncompressed
@@ -16,91 +16,96 @@ Inductive compressionMethod : Set :=
   | CompressionETC2
   | CompressionEAC
   | CompressionASTC : nat → nat → compressionMethod
-  | CompressionCustom : descriptor → nat → nat → nat → nat → compressionMethod.
+  | CompressionCustom :
+    ∀ (d : descriptor) 
+      (blockSizeX : nat) 
+      (blockSizeY : nat) 
+      (identifier : nat) 
+      (align : nat), 0 < align → compressionMethod.
 
 Definition compressionMethodDescriptor (c : compressionMethod) :=
   match c with
-  | CompressionUncompressed     => "UNCOMPRESSED"
-  | CompressionBC1              => "BC1"
-  | CompressionBC2              => "BC2"
-  | CompressionBC3              => "BC3"
-  | CompressionBC4              => "BC4"
-  | CompressionBC5              => "BC5"
-  | CompressionBC6              => "BC6"
-  | CompressionBC7              => "BC7"
-  | CompressionETC1             => "ETC1"
-  | CompressionETC2             => "ETC2"
-  | CompressionEAC              => "EAC"
-  | CompressionASTC _ _         => "ASTC"
-  | CompressionCustom c _ _ _ _ => c
+  | CompressionUncompressed       => "UNCOMPRESSED"
+  | CompressionBC1                => "BC1"
+  | CompressionBC2                => "BC2"
+  | CompressionBC3                => "BC3"
+  | CompressionBC4                => "BC4"
+  | CompressionBC5                => "BC5"
+  | CompressionBC6                => "BC6"
+  | CompressionBC7                => "BC7"
+  | CompressionETC1               => "ETC1"
+  | CompressionETC2               => "ETC2"
+  | CompressionEAC                => "EAC"
+  | CompressionASTC _ _           => "ASTC"
+  | CompressionCustom c _ _ _ _ _ => c
   end.
 
 Definition compressionBlockSizeX (c : compressionMethod) : nat :=
   match c with
-  | CompressionUncompressed     => 0
-  | CompressionBC1              => 4
-  | CompressionBC2              => 4
-  | CompressionBC3              => 4
-  | CompressionBC4              => 4
-  | CompressionBC5              => 4
-  | CompressionBC6              => 4
-  | CompressionBC7              => 4
-  | CompressionETC1             => 4
-  | CompressionETC2             => 4
-  | CompressionEAC              => 4
-  | CompressionASTC x _         => x
-  | CompressionCustom _ x _ _ _ => x
+  | CompressionUncompressed       => 0
+  | CompressionBC1                => 4
+  | CompressionBC2                => 4
+  | CompressionBC3                => 4
+  | CompressionBC4                => 4
+  | CompressionBC5                => 4
+  | CompressionBC6                => 4
+  | CompressionBC7                => 4
+  | CompressionETC1               => 4
+  | CompressionETC2               => 4
+  | CompressionEAC                => 4
+  | CompressionASTC x _           => x
+  | CompressionCustom _ x _ _ _ _ => x
   end.
 
 Definition compressionBlockSizeY (c : compressionMethod) : nat :=
   match c with
-  | CompressionUncompressed     => 0
-  | CompressionBC1              => 4
-  | CompressionBC2              => 4
-  | CompressionBC3              => 4
-  | CompressionBC4              => 4
-  | CompressionBC5              => 4
-  | CompressionBC6              => 4
-  | CompressionBC7              => 4
-  | CompressionETC1             => 4
-  | CompressionETC2             => 4
-  | CompressionEAC              => 4
-  | CompressionASTC _ y         => y
-  | CompressionCustom _ _ y _ _ => y
+  | CompressionUncompressed       => 0
+  | CompressionBC1                => 4
+  | CompressionBC2                => 4
+  | CompressionBC3                => 4
+  | CompressionBC4                => 4
+  | CompressionBC5                => 4
+  | CompressionBC6                => 4
+  | CompressionBC7                => 4
+  | CompressionETC1               => 4
+  | CompressionETC2               => 4
+  | CompressionEAC                => 4
+  | CompressionASTC _ y           => y
+  | CompressionCustom _ _ y _ _ _ => y
   end.
 
 Definition compressionSectionIdentifier (c : compressionMethod) : nat :=
   match c with
-  | CompressionUncompressed     => 0
-  | CompressionBC1              => 0
-  | CompressionBC2              => 0
-  | CompressionBC3              => 0
-  | CompressionBC4              => 0
-  | CompressionBC5              => 0
-  | CompressionBC6              => 0
-  | CompressionBC7              => 0
-  | CompressionETC1             => 0
-  | CompressionETC2             => 0
-  | CompressionEAC              => 0
-  | CompressionASTC _ _         => 0
-  | CompressionCustom _ _ _ i _ => i
+  | CompressionUncompressed       => 0
+  | CompressionBC1                => 0
+  | CompressionBC2                => 0
+  | CompressionBC3                => 0
+  | CompressionBC4                => 0
+  | CompressionBC5                => 0
+  | CompressionBC6                => 0
+  | CompressionBC7                => 0
+  | CompressionETC1               => 0
+  | CompressionETC2               => 0
+  | CompressionEAC                => 0
+  | CompressionASTC _ _           => 0
+  | CompressionCustom _ _ _ i _ _ => i
   end.
 
 Definition compressionBlockAlignment (c : compressionMethod) : nat :=
   match c with
-  | CompressionUncompressed     => 0
-  | CompressionBC1              => 8
-  | CompressionBC2              => 16
-  | CompressionBC3              => 16
-  | CompressionBC4              => 8
-  | CompressionBC5              => 16
-  | CompressionBC6              => 16
-  | CompressionBC7              => 16
-  | CompressionETC1             => 16
-  | CompressionETC2             => 16
-  | CompressionEAC              => 16
-  | CompressionASTC _ _         => 16
-  | CompressionCustom _ _ _ _ a => a
+  | CompressionUncompressed       => 0
+  | CompressionBC1                => 8
+  | CompressionBC2                => 16
+  | CompressionBC3                => 16
+  | CompressionBC4                => 8
+  | CompressionBC5                => 16
+  | CompressionBC6                => 16
+  | CompressionBC7                => 16
+  | CompressionETC1               => 16
+  | CompressionETC2               => 16
+  | CompressionEAC                => 16
+  | CompressionASTC _ _           => 16
+  | CompressionCustom _ _ _ _ a _ => a
   end.
 
 Definition compressionIsNotCompressed (c : compressionMethod) : Prop :=
